PiLL/PiLL/Alt.lean
@@ -1,0 +1,424 @@
+import Mathlib.Data.Finset.Basic
+import Mathlib.Data.Finset.Card
+import Mathlib.Data.Finset.Fold
+
+-- inductive Typing : Finset (Nat) → Prop where
+--   | global {Γ : Finset Nat} :
+--       Typing Γ
+
+--   | bot {Γ : Finset Nat} {x : Nat} :
+--       Typing Γ →
+--       ----------------
+--       Typing (Γ ∪ {x})
+
+--   | parr {Γ : Finset Nat} {x y : Nat} :
+--     Typing (Γ ∪ {y} ∪ {x}) → Typing (Γ ∪ {x + y})
+
+-- inductive TypingStep : {𝒢 : Finset Nat} → Typing 𝒢 → (l : List Nat) →
+--   {𝒢' : Finset Nat} → Typing 𝒢' → Prop where
+--    | bot
+--       {Γ : Finset Nat} {x : Nat} (𝒟 : Typing (Γ)) :
+--       TypingStep (Typing.bot 𝒟) ([x]) (𝒟)
+
+--   | parr
+--       {Γ : Finset Nat} {x y : Nat} (𝒟 : Typing (Γ ∪ {y} ∪ {x})) :
+--       ------------------------------------------------------------
+--       TypingStep (Typing.parr 𝒟) [x, y] 𝒟
+
+-- notation:50 𝒟 " -[" l "]-> " 𝒟' => TypingStep 𝒟 l 𝒟'
+
+-- example {Γ : Finset ℕ} {x y : ℕ}
+--   (ℱ : Typing (Γ ∪ {x + y})) (ℱ' : Typing (Γ ∪ {y} ∪ {x})) :
+--   ℱ -[[x, y]]-> ℱ' := by
+--   apply TypingStep.parr
+
+
+
+
+/- Processes -/
+abbrev PName := Nat
+
+inductive Proc : Type where
+  | tensor  (x y : PName) (P : Proc)   -- x[y].P
+  | parr    (x y : PName) (P : Proc)   -- x(y).P
+  | one     (x : PName) (P : Proc)     -- x[].P
+  | bot     (x : PName) (P : Proc)     -- x().P
+  | cut     (x y : PName) (P : Proc)   -- 𝒗xy P
+  | par     (P Q : Proc)               -- P | Q
+  | nil                                -- 𝟘
+deriving DecidableEq
+
+abbrev Renaming := PName → PName
+
+def rename (ρ : Renaming) : Proc → Proc
+  | .tensor x y P => .tensor (ρ x) (ρ y) (rename ρ P)
+  | .parr x y P   => .parr (ρ x) (ρ y) (rename ρ P)
+  | .one x P      => .one (ρ x) (rename ρ P)
+  | .bot x P      => .bot (ρ x) (rename ρ P)
+  | .cut x y P    => .cut (ρ x) (ρ y) (rename ρ P)
+  | .par P Q      => .par (rename ρ P) (rename ρ Q)
+  | .nil          => .nil
+
+@[simp]
+def Proc.fNames : Proc → Finset PName
+  | .tensor x y P         => {x} ∪ (P.fNames \ {y})
+  | .parr x y P           => {x} ∪ (P.fNames \ {y})
+  | .one x P              => {x} ∪ P.fNames
+  | .bot x P              => {x} ∪ P.fNames
+  | .cut x y P            => P.fNames \ {x, y}
+  | .par P Q              => P.fNames ∪ Q.fNames
+  | .nil                  => {}
+
+@[simp]
+def Proc.names : Proc → Finset PName
+  | .tensor x y P => {x, y} ∪ P.names
+  | .parr x y P   => {x, y} ∪ P.names
+  | .one x P      => {x} ∪ P.names
+  | .bot x P      => {x} ∪ P.names
+  | .cut x y P    => {x, y} ∪ P.names
+  | .par P Q      => P.names ∪ Q.names
+  | .nil          => {}
+
+def freshName (s : Finset Nat) : PName :=
+  (Finset.fold Nat.max 0 id s) + 1
+
+def renameBound old new P := rename (fun curr => if curr == old then new else curr) P
+
+def renameBound2 old1 old2 new1 new2 P := renameBound old2 new2 (renameBound old1 new1 P)
+
+-- Only bound names should be renamed and free names should match exactly
+inductive AlphaEq : Proc → Proc → Prop where
+  | nil : AlphaEq .nil .nil
+
+  | par {P1 Q1 P2 Q2 : Proc} :
+      AlphaEq P1 Q1 → AlphaEq P2 Q2 → AlphaEq (.par P1 P2) (.par Q1 Q2)
+
+  | tensor {P Q : Proc} {x y x' y' : PName} : -- All PNames are free
+      AlphaEq P Q → AlphaEq (.tensor x y P) (.tensor x' y' Q)
+      → x = x' → y = y' → AlphaEq (.tensor x y P) (.tensor x' y' Q)
+
+  | one {P Q : Proc} {x x' : PName} : -- Both PNames are free
+      AlphaEq P Q → x = x' → AlphaEq (.one x P) (.one x' Q)
+
+  | bot {P Q : Proc} {x x' : PName} : -- Both PNames are free
+      AlphaEq P Q → x = x' → AlphaEq (.bot x P) (.bot x' Q)
+
+  | parr {P Q : Proc} {x y x' y' : PName} -- x x' are Free, y y' are bound
+      (w : PName) (hFresh : w ∉ P.names ∪ Q.names) :
+        AlphaEq (renameBound y w P) (renameBound y' w Q) → x = x' →
+        AlphaEq (.parr x y P) (.parr x' y' Q)
+
+  | cut {P Q : Proc} {x y x' y' : PName} -- x y x' y' are all bound
+      (w1 w2 : PName) (hFresh : w1 ∉ P.names ∪ Q.names ∧ w2 ∉ P.names ∪ Q.names) :
+        AlphaEq (renameBound2 x y w1 w2 P) (renameBound2 x' y' w1 w2 Q) →
+        AlphaEq (.cut x y P) (.cut x' y' Q)
+
+/- TYPES -/
+abbrev Atom := Nat
+
+inductive Types : Type where
+  | atom      (a : Atom)      -- named type, like A, B, ...
+  | atomDual  (a : Atom)      -- dual of a named type
+  | tensor    (A B : Types)   -- t₁ ⊗ t₂ (send)
+  | parr      (A B : Types)   -- t₁ ⅋ t₂ (receive)
+  | one                       -- 𝟙 (empty output, unit for ⊗)
+  | bot                       -- ⊥ (empty send, unit for ⅋)
+deriving DecidableEq
+
+def Types.pos : Types → Prop
+  | atom _ => True
+  | one => True
+  | tensor _ _ => True
+  -- | oplus _ _ => True
+  -- | bang _ => True
+  -- | zero => True
+  | _ => False
+
+def Types.neg : Types → Prop
+  | atomDual _ => True
+  | bot => True
+  | parr _ _ => True
+  -- | top => True
+  -- | .with _ _ => True
+  -- | quest _ => True
+  | _ => False
+
+instance Types.posDecidable (A : Types) : Decidable A.pos := by
+  unfold Types.pos
+  split <;> infer_instance
+
+instance Types.negDecidable (A : Types) : Decidable A.neg := by
+  unfold Types.neg
+  split <;> infer_instance
+
+@[simp]
+def Types.dual : Types → Types
+  | .tensor A B => .parr (dual A) (dual B)
+  | .parr A B   => .tensor (dual A) (dual B)
+  | .one        => .bot
+  | .bot        => .one
+  | .atom a     => .atomDual a
+  | .atomDual a => .atom a
+
+@[simp]
+theorem Types.dual.neq (A : Types) : A ≠ Types.dual A := by
+  cases A <;> simp [dual]
+
+@[simp]
+theorem dual.inj (A B : Types) : A.dual = B.dual ↔ A = B := by
+  induction A generalizing B <;> cases B <;> simp [Types.dual, *]
+
+@[simp]
+theorem dual.involution (A : Types) : A.dual.dual = A := by
+  induction A <;> simp [*]
+
+
+/- ENVIRONMENTS -/
+abbrev Env := Finset (PName × Types)
+@[simp] theorem Env.merge_unitR (Δ : Env) : Δ ∪ ∅ = Δ := by simp
+
+@[simp] theorem Env.merge_unitL (Δ : Env) : ∅ ∪ Δ = Δ := by simp
+
+@[simp] theorem Env.merge_comm (Δ Γ : Env) : Δ ∪ Γ = Γ ∪ Δ := by simp [Finset.union_comm]
+
+@[simp] theorem Env.merge_assoc (Δ Γ Ε : Env) : (Δ ∪ Γ) ∪ Ε = Δ ∪ (Γ ∪ Ε) := by simp
+
+@[simp] lemma Env.merge_swap_last (Γ Δ Ξ : Env) : (Γ ∪ Δ) ∪ Ξ = (Γ ∪ Ξ) ∪ Δ := by
+  rw [Env.merge_comm, ←Env.merge_assoc]
+  conv => lhs ; lhs ; rw [Env.merge_comm]
+
+
+/- HYPER ENVIRONMENTS -/
+abbrev HyperEnv := Finset (Env)
+
+@[simp] theorem HyperEnv.merge_unitL (𝒢 : HyperEnv) : ∅ ∪ 𝒢 = 𝒢 := by simp
+
+@[simp] theorem HyperEnv.merge_unitR (𝒢 : HyperEnv) : 𝒢 ∪ ∅ = 𝒢 := by simp
+
+@[simp] theorem HyperEnv.merge_comm (𝒢 ℋ : HyperEnv) : 𝒢 ∪ ℋ = ℋ ∪ 𝒢 := by simp [Finset.union_comm]
+
+@[simp] theorem HyperEnv.merge_assoc (𝒢 ℋ 𝒦 : HyperEnv) : (𝒢 ∪ ℋ) ∪ 𝒦 = 𝒢 ∪ (ℋ ∪ 𝒦) := by simp
+
+
+/- TYPINGS -/
+inductive Typing : HyperEnv → Proc → Prop where
+  | mix₀ :
+      -----------------
+      Typing ∅ Proc.nil
+
+  | mix {𝒢 ℋ : HyperEnv} {P Q : Proc} :
+      Typing 𝒢 P → Typing ℋ Q →
+      --------------------------
+      Typing (𝒢 ∪ ℋ) (Proc.par P Q)
+
+  | cut (𝒢 : HyperEnv) (Γ Δ : Env) (P : Proc) (x y : PName) (A : Types) :
+      Typing (𝒢 ∪ {Γ ∪ {(x, A)}} ∪ {Δ ∪ {(y, A.dual)}}) P →
+      ------------------------------------------------------
+      Typing (𝒢 ∪ {Γ ∪ Δ}) (Proc.cut x y P)
+
+  | one {P : Proc} {x : PName} :
+      Typing ∅ P →
+      ----------------------------------------
+      Typing {{(x, Types.one)}} (Proc.one x P)
+
+  | tensor {Γ Δ : Env} {P : Proc} {x y : PName} {B A : Types} :
+      Typing ({Γ ∪ {(y, A)}} ∪ {Δ ∪ {(x, B)}}) P →
+      --------------------------------------------------------------
+      Typing ({Γ ∪ Δ ∪ {(x, Types.tensor A B)}}) (Proc.tensor x y P)
+
+  | bot {Γ : Env} {P : Proc} {x : PName} :
+      Typing {Γ} P →
+      --------------------------------------------
+      Typing {Γ ∪ {(x, Types.bot)}} (Proc.bot x P)
+
+  | parr {Γ : Env} {P : Proc} {x y : PName} {A B : Types} :
+      Typing {Γ ∪ {(y, A)} ∪ {(x, B)}} P →
+      -------------------------------------------------------
+      Typing {Γ ∪ {(x, (Types.parr A B))}} (Proc.parr x y P)
+
+
+/- LABELS -/
+inductive Act : Type
+  | one     (x : PName)     -- x[]
+  | bot     (x : PName)     -- x()
+  | tensor  (x y : PName)   -- x[y]
+  | parr    (x y : PName)   -- x(y)
+deriving Repr, DecidableEq
+
+inductive Lbl : Type
+  | tau                       -- τ
+  | act   (a : Act)           -- l, for l ∈ Act
+  | par   (l l' : Act)        -- l | l' for l, l' ∈ Act
+deriving Repr, DecidableEq
+
+abbrev Lbls := List Lbl
+
+instance : Coe Act Lbl := ⟨Lbl.act⟩
+
+@[simp]
+def getNamesOfLbl (func : Act → Finset PName) : Lbl → Finset PName
+  | .tau        => ∅                  -- names for τ
+  | .act a      => func a             -- names for l with l ∈ Act
+  | .par l l'   => func l ∪ func l'   -- names for l | l' with l, l' ∈ Act
+
+@[simp]
+def fNamesAct : Act -> Finset PName -- free names for a given action
+  | .one x | .bot x | .tensor x _ | .parr x _ => {x}
+
+@[simp]
+def Lbl.fNames : Lbl → Finset PName :=
+  getNamesOfLbl fNamesAct
+
+@[simp]
+def iNamesAct : Act → Finset PName -- introduced names for a given action
+  | .one _ | .bot _          => {}
+  | .tensor _ y | .parr _ y => {y}
+
+@[simp]
+def Lbl.iNames : Lbl → Finset PName :=
+  getNamesOfLbl iNamesAct
+
+@[simp]
+def Lbl.fresh (xs : List PName) (l : Lbl) :=
+  ∀ n ∈ xs, n ∉ l.fNames ∪ l.iNames
+
+
+/- TYPING TRANSITIONS-/
+-- FIXME: Make arrow based instead premise → premise → ... → premise → conlcusion
+inductive TypingStep : {𝒢 : HyperEnv} → {P : Proc} → Typing 𝒢 P → (l : Lbl) →
+  {𝒢' : HyperEnv} → {P : Proc} → Typing 𝒢' P → Prop where
+  | one
+      {P : Proc} {x : PName} {𝒟 : Typing ∅ P} :
+      TypingStep (Typing.one 𝒟) (Lbl.act (Act.one x)) 𝒟
+
+  | tensor
+      {Γ Δ : Env} {P : Proc} {x x': PName} {A B : Types}
+      {𝒟 : Typing ({Γ ∪ {(x', A)}} ∪ {Δ ∪ {(x, B)}}) P} :
+      TypingStep (Typing.tensor 𝒟) (Lbl.act (Act.tensor x x')) 𝒟
+
+  | bot
+      {Γ : Env} {P : Proc} {x : PName} (𝒟 : Typing {Γ} P) :
+      TypingStep (Typing.bot (x := x) 𝒟) (Lbl.act (Act.bot x)) (𝒟)
+
+  | parr
+      {Γ : Env} {P : Proc} {x x' : PName} {A B : Types} :
+      (𝒟 : Typing {Γ ∪ {(x', A)} ∪ {(x, B)}} P) →
+      -----------------------------------------------------------
+      TypingStep (Typing.parr 𝒟) (Lbl.act (Act.parr x x')) 𝒟
+
+  | par₁
+      {𝒢 ℋ 𝒢': HyperEnv} {P Q P' : Proc} {l : Lbl}
+      {𝒟 : Typing 𝒢 P} {𝒟' : Typing 𝒢' P'} {ℰ : Typing ℋ Q} :
+      TypingStep 𝒟 l 𝒟' → (l.iNames) ∩ (Q.fNames) = ∅ →
+      --------------------------------------------------
+      TypingStep (Typing.mix 𝒟 ℰ) l (Typing.mix 𝒟' ℰ)
+
+  | par₂
+      {𝒢 ℋ ℋ': HyperEnv} {P Q Q' : Proc} {l : Lbl}
+      {𝒟 : Typing 𝒢 P} {ℰ : Typing ℋ Q} {ℰ' : Typing ℋ' Q'} :
+      TypingStep ℰ l ℰ' → (l.iNames) ∩ (P.fNames) = ∅ →
+      --------------------------------------------------
+      TypingStep (Typing.mix 𝒟 ℰ) l (Typing.mix 𝒟 ℰ')
+
+  | syn
+      {𝒢 𝒢' ℋ ℋ' : HyperEnv} {P P' Q Q' : Proc} {a a' : Act}
+      {𝒟 : Typing 𝒢 P} {𝒟' : Typing 𝒢' P'}
+      {ℰ : Typing ℋ Q} {ℰ' : Typing ℋ' Q'} :
+      (h₁ : TypingStep 𝒟 a 𝒟') → TypingStep ℰ a' ℰ' →
+      ((Lbl.par a a').iNames ∩ (Proc.par P Q).fNames) = ∅ →
+      ---------------------------------------------------------------
+      TypingStep (Typing.mix 𝒟 ℰ) (Lbl.par a a') (Typing.mix 𝒟' ℰ')
+
+  | alpha_equiv
+      {𝒢 𝒢' : HyperEnv} {P Q Q' : Proc} {l : Lbl}
+      {𝒟 : Typing 𝒢 P} {ℰ : Typing 𝒢 Q} {ℰ' : Typing 𝒢' Q'} :
+      AlphaEq P Q → TypingStep ℰ l ℰ' →
+      --------------------------------------------------------
+      TypingStep 𝒟 l ℰ'
+
+  | one_bot
+      {𝒢: HyperEnv} {Γ : Env} {P P' : Proc} {x y : PName}
+      {𝒟 : Typing (𝒢 ∪ {{(x, Types.one)}} ∪ {Γ ∪ {(y, Types.bot)}}) P}
+      {𝒟' : Typing (𝒢 ∪ {Γ}) P'} :
+      TypingStep 𝒟 (Lbl.par (Act.one x) (Act.bot y)) 𝒟' →
+      -----------------------------------------------------------------
+      TypingStep (Typing.cut 𝒢 ∅ Γ P x y (Types.one) 𝒟) (Lbl.tau) 𝒟'
+
+  | tensor_parr
+      {𝒢 : HyperEnv} {Γ Δ Ξ : Env} {P P' : Proc} {x y x' y' : PName} {A B : Types}
+      {𝒟 : Typing (𝒢 ∪ {(Γ ∪ Δ) ∪ {(x, Types.tensor A B)}} ∪
+        {Ξ ∪ {(y, Types.parr A.dual B.dual)}}) P
+      }
+      {𝒟' : Typing ((𝒢 ∪ {Γ ∪ {(x, B)}}) ∪ {Δ ∪
+        {(x', A)}} ∪ {(Ξ ∪ {(y, B.dual)}) ∪ {(y', A.dual)}}) P'
+      } :
+      TypingStep 𝒟 (Lbl.par (Act.tensor x x') (Act.parr y y')) 𝒟' →
+      ----------------------------------------------------------------------------
+      TypingStep
+        (Typing.cut 𝒢 (Γ ∪ Δ) Ξ P x y (Types.tensor A B) 𝒟)
+        (Lbl.tau)
+        (by constructor
+          -- let inner := Typing.cut (𝒢 ∪ {Γ ∪ {(x, B)}}) Δ (Ξ ∪ {(y, B.dual)}) P' x' y' A 𝒟'
+          -- conv at inner => lhs ; rhs ; rhs ; rw [← Env.merge_assoc]
+          -- exact Typing.cut 𝒢 Γ (Δ ∪ Ξ) (Proc.cut x' y' P') x y B inner
+        )
+
+  | res
+      {𝒢 𝒢': HyperEnv} {Γ Γ' Δ Δ' : Env} {P P' : Proc}
+      {x y : PName} {A : Types} {l : Lbl}
+      {𝒟 : Typing (𝒢 ∪ {Γ ∪ {(x, A)}} ∪ {Δ ∪ {(y, A.dual)}}) P}
+      {𝒟' : Typing (𝒢' ∪ {Γ' ∪ {(x, A)}} ∪ {Δ' ∪ {(y, A.dual)}}) P'}
+      (h : TypingStep 𝒟 l 𝒟')
+      (disj : l.fresh [x, y]) :
+      ----------------------------------------------------------------------------
+      TypingStep (Typing.cut 𝒢 Γ Δ P x y A 𝒟) l (Typing.cut 𝒢' Γ' Δ' P' x y A 𝒟')
+
+
+
+
+
+
+
+example {Γ : Env} {P : Proc} {x y : PName}
+  (ℱ : Typing {Γ ∪ {(x, (Types.parr Types.bot Types.bot))}} (Proc.parr x y P))
+  (ℱ' : Typing {Γ ∪ {(y, Types.bot)} ∪ {(x, Types.bot)}} P) :
+  TypingStep ℱ (Lbl.act (Act.parr x y)) ℱ' := by
+  apply TypingStep.parr
+
+theorem ℰ (Γ Γ' : Env) (x x' : PName) (A B : Types) (Q : Proc)
+  (ℰ' : Typing ({Γ' ∪ {(x', A)}} ∪ {Γ ∪ {(x, B)}}) Q) :
+  Typing {Γ' ∪ Γ ∪ {(x, Types.tensor A B)}} (Proc.tensor x x' Q) := by
+  apply Typing.tensor
+  exact ℰ'
+
+theorem ℱ (Δ : Env) (R : Proc) (y y' z : PName) (A B : Types)
+  (ℱ' : Typing {Δ ∪ {(y', A.dual)} ∪ {(y, B.dual)}} R) :
+  Typing
+    {Δ ∪ {(y, Types.parr A.dual B.dual)} ∪ {(z, Types.bot)}}
+    (Proc.parr y y' (Proc.bot z R)) := by
+  rw [Env.merge_swap_last]
+  apply Typing.parr
+  rw [Env.merge_assoc, Env.merge_swap_last]
+  apply Typing.bot
+  rw [← Env.merge_assoc]
+  exact ℱ'
+
+theorem 𝒟 (Γ Γ' Δ : Env) (Q R : Proc) (x x' y y' z) (A B : Types)
+  (ℰ' : Typing ({Γ' ∪ {(x', A)}} ∪ {Γ ∪ {(x, B)}}) Q)
+  (ℱ' : Typing {Δ ∪ {(y', A.dual)} ∪ {(y, B.dual)}} R) :
+  Typing
+    {Γ' ∪ Γ ∪ Δ ∪ {(z, Types.bot)}}
+    (Proc.cut x y (Proc.par (Proc.tensor x x' Q) (Proc.parr y y' (Proc.bot z R)))) := by
+    let t := Typing.cut ∅ (Γ' ∪ Γ) (Δ ∪ {(z, Types.bot)})
+      (Proc.par (Proc.tensor x x' Q) (Proc.parr y y' (Proc.bot z R))) x y (Types.tensor A B)
+    repeat rw [HyperEnv.merge_unitL] at t
+    rw [Env.merge_assoc]
+    apply t
+    apply Typing.mix
+    · apply Typing.tensor
+      exact ℰ'
+    · apply Typing.parr
+      rw [Env.merge_assoc, Env.merge_swap_last]
+      apply Typing.bot
+      rw [← Env.merge_assoc]
+      exact ℱ'
